Add get_ident to Name class

pcuic/theories/Name.v
@@ -8,17 +8,26 @@ From Template Require Import BasicAst.
 Class Name := {
   name : Set ;
   nNamed : string -> name ;
-  nAnon : name
+  nAnon : name ;
+  get_ident : name -> string
 }.
+
+Definition basic_get_ident (n : BasicAst.name) : string :=
+  match n with
+  | BasicAst.nAnon => "XX"
+  | BasicAst.nNamed i => i
+  end.
 
 Local Instance BasicName : Name := {
   name := BasicAst.name ;
   nNamed := BasicAst.nNamed ;
-  nAnon := BasicAst.nAnon
+  nAnon := BasicAst.nAnon ;
+  get_ident := basic_get_ident
 }.
 
 Local Instance Nameless : Name := {
   name := unit ;
   nNamed s := tt ;
-  nAnon := tt
+  nAnon := tt ;
+  get_ident _ := "XX"%string
 }.
